Use `suffices` instead of direct proof reconstruction

Extraction/Core.lean
@@ -27,24 +27,13 @@ def extractExpr? (target expr : Expr) : GoalM (Option Expr) := do
     else
       return none
 
-def extractMain? (target : Expr) : Sketch → GoalM (Option Expr)
-  | .minAST =>
+-- Note: This is expected to be run in the context of the failed grind goal, and with `target`
+--       being internalized.
+def extract? (target : Expr) : Sketch → GoalM (Option Expr)
+  | .minAST => do
     extractMinAST target
   | .expr e => do
     let e ← shareCommon e
     extractExpr? target e
   | _ =>
     throwError "`grind extract` currently only supports the `min_ast` and expression sketches"
-
-structure Extracted where
-  /-- The result of extraction: the extracted term, equivalent to the proof goal. -/
-  result     : Expr
-  /-- Proves `result = target`/`result ≍ target`. -/
-  eqHEqProof : Expr
-
--- Note: This is expected to be run in the context of the failed grind goal, and with `target`
---       being internalized.
-def extract? (target : Expr) (sketch : Sketch) : GoalM (Option Extracted) := do
-  let some result ← extractMain? target sketch | return none
-  let eqHEqProof ← mkEqHEqProof result target
-  return some { result, eqHEqProof }
